cleaning up map utils

disk-betree/BlockCache.dfy
@@ -1,11 +1,35 @@
 abstract module BlockCache {
-  type Constants
-  type Variables(!new)<T>
-
+  import MissingLibrary
+    
   type Reference(!new,==)
 
   type View<T> = imap<Reference, T>
+  type ReferenceTree = imap<Reference, set<Reference>>
+
+  function Root(k: Constants) : Reference
+
+  type Constants
+  datatype Variables<T> = Variables(view: View, reftree: ReferenceTree)
     
+  type Lookup = seq<Reference>
+    
+  predicate LookupIsValid(k: Constants, s: Variables, lookup: Lookup)
+  {
+    && |lookup| > 0
+    && lookup[0] == Root(k)
+    && (forall i :: 0 <= i < |lookup|-1 ==> lookup[i+1] in s.reftree[lookup[i]])
+  }
+
+  predicate ReachableReference(k: Constants, s: Variables, ref: Reference)
+  {
+    exists lookup :: LookupIsValid(k, s, lookup) && Last(lookup) == ref
+  }
+
+  function LiveReferences(k: Constants, s: Variables) : set<Reference> {
+    set ref | ReachableReference(k, s, ref)
+  }
+
+  
   function ViewOf<T>(k: Constants, s: Variables) : View
   
   // function Read<T>(k: Constants, s: Variables, ref: Reference) : T
@@ -22,8 +46,8 @@ abstract module BlockCache {
     
   predicate Apply(k: Constants, s: Variables, s': Variables, op: CacheOp)
     ensures Apply(k, s, s', op) ==> ViewOf(k, s') == ApplyToView(ViewOf(k, s), op)
-    ensures op.AllocOp? && Apply(k, s, s', op) ==> op.ref !in ViewOf(k, s)
-    ensures op.WriteOp? && Apply(k, s, s', op) ==> op.ref in ViewOf(k, s)
+    ensures op.AllocOp? && Apply(k, s, s', op) ==> op.ref !in LiveReferences(k, s)
+    ensures op.WriteOp? && Apply(k, s, s', op) ==> op.ref in LiveReferences(k, s)
     
   predicate Apply2(k: Constants, s: Variables, s': Variables, op1: CacheOp, op2: CacheOp)
     ensures Apply2(k, s, s', op1, op2) ==> ViewOf(k, s') == ApplyToView(ApplyToView(ViewOf(k, s), op1), op2)
@@ -32,8 +56,13 @@ abstract module BlockCache {
       && Apply(k, s, sint, op1)
       && Apply(k, sint, s', op2)
   }
-    
-  function Root(k: Constants) : Reference
 
+  predicate GC(k: Constants, s: Variables, s': Variables, ref: Reference) {
+    && ref !in LiveReferences(k, s)
+    && ref in ViewOf(k, s)
+    && s'.view == MapRemove(s, ref)
+    && s'.reftree == s.reftree
+  }
+  
   predicate Init(k: Constants, s: Variables)
 }
