lib/map_utils.dfy
@@ -1,26 +1,26 @@
 module Map_Utils {
 
 	// Requires disjoint domains and delivers predictable result.
-	function method {:opaque} disjoint_union<U,T>(mapa: map<U,T>, mapb: map<U,T>) : map<U,T>
+	function method {:opaque} MapDisjointUnion<U,T>(mapa: map<U,T>, mapb: map<U,T>) : map<U,T>
 		requires mapa.Keys !! mapb.Keys;
-		ensures disjoint_union(mapa, mapb).Keys == mapa.Keys + mapb.Keys;
-		ensures mapa.Keys != {} || mapb.Keys != {} ==> disjoint_union(mapa, mapb).Keys != {};
-		ensures forall k :: k in mapa.Keys ==> mapa[k] == disjoint_union(mapa, mapb)[k];
-		ensures forall k :: k in mapb.Keys ==> mapb[k] == disjoint_union(mapa, mapb)[k];
+		ensures MapDisjointUnion(mapa, mapb).Keys == mapa.Keys + mapb.Keys;
+		ensures mapa.Keys != {} || mapb.Keys != {} ==> MapDisjointUnion(mapa, mapb).Keys != {};
+		ensures forall k :: k in mapa.Keys ==> mapa[k] == MapDisjointUnion(mapa, mapb)[k];
+		ensures forall k :: k in mapb.Keys ==> mapb[k] == MapDisjointUnion(mapa, mapb)[k];
 	{
 		map x : U | (x in mapa.Keys + mapb.Keys) :: if x in mapa then mapa[x] else mapb[x]
 	}
 
 	// Requires disjoint domains and delivers predictable result.
-	function method {:opaque} disjoint_union3<U,T>(mapa: map<U,T>, mapb: map<U,T>, mapc: map<U,T>) : map<U,T>
+	function method {:opaque} MapDisjointUnion3<U,T>(mapa: map<U,T>, mapb: map<U,T>, mapc: map<U,T>) : map<U,T>
 		requires mapa.Keys !! mapb.Keys !! mapc.Keys;
-		ensures disjoint_union3(mapa, mapb, mapc).Keys == mapa.Keys + mapb.Keys + mapc.Keys;
-		ensures mapa.Keys != {} || mapb.Keys != {} || mapc.Keys != {} ==> disjoint_union3(mapa, mapb, mapc).Keys != {};
-		ensures forall k :: k in mapa.Keys ==> mapa[k] == disjoint_union3(mapa, mapb, mapc)[k];
-		ensures forall k :: k in mapb.Keys ==> mapb[k] == disjoint_union3(mapa, mapb, mapc)[k];
-		ensures forall k :: k in mapc.Keys ==> mapc[k] == disjoint_union3(mapa, mapb, mapc)[k];
-		ensures disjoint_union3(mapa, mapb, mapc) == disjoint_union(mapa, disjoint_union(mapb, mapc))
-			                                        == disjoint_union(disjoint_union(mapa, mapb), mapc);
+		ensures MapDisjointUnion3(mapa, mapb, mapc).Keys == mapa.Keys + mapb.Keys + mapc.Keys;
+		ensures mapa.Keys != {} || mapb.Keys != {} || mapc.Keys != {} ==> MapDisjointUnion3(mapa, mapb, mapc).Keys != {};
+		ensures forall k :: k in mapa.Keys ==> mapa[k] == MapDisjointUnion3(mapa, mapb, mapc)[k];
+		ensures forall k :: k in mapb.Keys ==> mapb[k] == MapDisjointUnion3(mapa, mapb, mapc)[k];
+		ensures forall k :: k in mapc.Keys ==> mapc[k] == MapDisjointUnion3(mapa, mapb, mapc)[k];
+		ensures MapDisjointUnion3(mapa, mapb, mapc) == MapDisjointUnion(mapa, MapDisjointUnion(mapb, mapc))
+			                                        == MapDisjointUnion(MapDisjointUnion(mapa, mapb), mapc);
 	{
 		map x : U | (x in mapa.Keys + mapb.Keys + mapc.Keys) ::
 			if x in mapa then mapa[x]
@@ -30,30 +30,77 @@ module Map_Utils {
 
 	// Doesn't require disjoint domains, but guarantees to take A's
 	// definition.
-	function method {:opaque} union_preferA<U,T>(mapa: map<U,T>, mapb: map<U,T>) : map<U,T>
-		ensures union_preferA(mapa, mapb).Keys == mapa.Keys + mapb.Keys;
-		ensures mapa.Keys != {} || mapb.Keys != {} ==> union_preferA(mapa, mapb).Keys != {};
-		ensures forall k :: k in mapa.Keys ==> mapa[k] == union_preferA(mapa, mapb)[k];
-		ensures forall k :: k in mapb.Keys - mapa.Keys ==> mapb[k] == union_preferA(mapa, mapb)[k];
+	function method {:opaque} MapUnionPreferA<U,T>(mapa: map<U,T>, mapb: map<U,T>) : (mapc:map<U,T>)
+		ensures mapc.Keys == mapa.Keys + mapb.Keys;
+    ensures forall k :: k in mapa.Keys ==> mapc[k] == mapa[k];
+    ensures forall k :: k in mapb.Keys - mapa.Keys ==> mapc[k] == mapb[k];
+    ensures forall k :: k in mapa.Keys && !(k in mapb.Keys) ==> mapc[k] == mapa[k]; // no-set-op translation is easier for Dafny
 	{
 		map x : U | (x in mapa.Keys + mapb.Keys) :: if x in mapa then mapa[x] else mapb[x]
 	}
 
+  function {:opaque} MapUnionPreferB<U,T>(mapa: map<U,T>, mapb: map<U,T>) : (mapc:map<U,T>)
+    ensures mapc.Keys == mapa.Keys + mapb.Keys;
+    ensures forall k :: k in mapb.Keys ==> mapc[k] == mapb[k];
+    ensures forall k :: k in mapa.Keys - mapb.Keys ==> mapc[k] == mapa[k];
+    ensures forall k :: k in mapa.Keys && !(k in mapb.Keys) ==> mapc[k] == mapa[k]; // no-set-op translation is easier for Dafny
+  {
+    map x : U | (x in mapa.Keys + mapb.Keys) :: if x in mapb then mapb[x] else mapa[x]
+  }
+  
 	// Doesn't require disjoint domains, and makes no promises about
 	// which it chooses on the intersection.
-	function method {:opaque} union<U,T>(mapa: map<U,T>, mapb: map<U,T>) : map<U,T>
-		ensures union(mapa, mapb).Keys == mapa.Keys + mapb.Keys;
-		ensures mapa.Keys != {} || mapb.Keys != {} ==> union(mapa, mapb).Keys != {};
-		ensures forall k :: k in mapa.Keys -mapb.Keys ==> mapa[k] == union(mapa, mapb)[k];
-		ensures forall k :: k in mapb.Keys - mapa.Keys ==> mapb[k] == union(mapa, mapb)[k];
+	function method {:opaque} MapUnion<U,T>(mapa: map<U,T>, mapb: map<U,T>) : map<U,T>
+		ensures MapUnion(mapa, mapb).Keys == mapa.Keys + mapb.Keys;
+		ensures mapa.Keys != {} || mapb.Keys != {} ==> MapUnion(mapa, mapb).Keys != {};
+		ensures forall k :: k in mapa.Keys -mapb.Keys ==> mapa[k] == MapUnion(mapa, mapb)[k];
+		ensures forall k :: k in mapb.Keys - mapa.Keys ==> mapb[k] == MapUnion(mapa, mapb)[k];
 		ensures forall k :: k in mapa.Keys * mapb.Keys ==>
-			mapb[k] == union(mapa, mapb)[k] || mapa[k] == union(mapa, mapb)[k];
+			mapb[k] == MapUnion(mapa, mapb)[k] || mapa[k] == MapUnion(mapa, mapb)[k];
 	{
-		union_preferA(mapa, mapb)
+		MapUnionPreferA(mapa, mapb)
 	}
 
   predicate IMapsTo<K,V>(m: imap<K, V>, k: K, v: V) {
     k in m && m[k] == v
   }
   
+  predicate MapsTo<K,V>(m: map<K, V>, k: K, v: V) {
+    k in m && m[k] == v
+  }
+
+  // Trigger bait
+  predicate InEmpty<K>(k: K) {
+    false
+  }
+  
+  function {:opaque} EmptyImap<K(!new),V>() : (e:imap<K,V>)
+    ensures e.Keys == iset{}
+  {
+    var v :| true;
+    imap k | InEmpty(k)  :: v
+  }
+  
+  function {:opaque} EmptyMap<K(!new),V>() : (e:map<K,V>)
+    ensures e.Keys == {}
+  {
+    var v :| true;
+    map k | k in {} && InEmpty(k) :: v
+  }
+  
+  function {:opaque} MapRemove<K,V>(m:map<K,V>, k:K) : (m':map<K,V>)
+    ensures m'.Keys == m.Keys - {k}
+    ensures forall j :: j in m' ==> m'[j] == m[j]
+  {
+    map j | j in m && j != k :: m[j]
+  }
+  
+  function {:opaque} ImapUnionPreferB<U,T>(mapa: imap<U,T>, mapb: imap<U,T>) : (mapc:imap<U,T>)
+    ensures mapc.Keys == mapa.Keys + mapb.Keys;
+    ensures forall k :: k in mapb.Keys ==> mapc[k] == mapb[k];
+    ensures forall k :: k in mapb.Keys - mapa.Keys ==> mapc[k] == mapb[k];
+    ensures forall k :: k in mapa.Keys && !(k in mapb.Keys) ==> mapc[k] == mapa[k]; // no-set-op translation is easier for Dafny
+  {
+    imap x : U | (x in mapa.Keys + mapb.Keys) :: if x in mapb then mapb[x] else mapa[x]
+  }
 }
