tla-tree/MissingLibrary.dfy
@@ -1,56 +1,5 @@
 module MissingLibrary {
 
-function /*{:opaque} XXX*/ Last<T>(s:seq<T>) : T
-    requires 0<|s|
-{
-    s[|s|-1]
-}
-
-function {:opaque} EmptyImap<K(!new),V>() : (e:imap<K,V>)
-    ensures e.Keys == iset{}
-{
-    var v :| true;
-    imap k | k in {} :: v
-}
-
-function {:opaque} EmptyMap<K(!new),V>() : (e:map<K,V>)
-    ensures e.Keys == {}
-{
-    var v :| true;
-    map k | k in {} :: v
-}
-
-function {:opaque} MapRemove<K,V>(m:map<K,V>, k:K) : (m':map<K,V>)
-    ensures m'.Keys == m.Keys - {k}
-    ensures forall j :: j in m' ==> m'[j] == m[j]
-{
-    map j | j in m && j != k :: m[j]
-}
-
-function {:opaque} SingletonImap<K,V>(k:K, v:V) : (m:imap<K,V>)
-    ensures m.Keys == iset {k}
-    ensures m[k] == v
-{
-    imap j | j == k :: v
-}
-
-function {:opaque} MapUnionPreferB<U,T>(mapa: map<U,T>, mapb: map<U,T>) : (mapc:map<U,T>)
-    ensures mapc.Keys == mapa.Keys + mapb.Keys;
-    ensures forall k :: k in mapb.Keys ==> mapc[k] == mapb[k];
-    ensures forall k :: k in mapb.Keys - mapa.Keys ==> mapc[k] == mapb[k];
-    ensures forall k :: k in mapa.Keys && !(k in mapb.Keys) ==> mapc[k] == mapa[k]; // no-set-op translation is easier for Dafny
-{
-    map x : U | (x in mapa.Keys + mapb.Keys) :: if x in mapb then mapb[x] else mapa[x]
-}
-
-function {:opaque} ImapUnionPreferB<U,T>(mapa: imap<U,T>, mapb: imap<U,T>) : (mapc:imap<U,T>)
-    ensures mapc.Keys == mapa.Keys + mapb.Keys;
-    ensures forall k :: k in mapb.Keys ==> mapc[k] == mapb[k];
-    ensures forall k :: k in mapb.Keys - mapa.Keys ==> mapc[k] == mapb[k];
-    ensures forall k :: k in mapa.Keys && !(k in mapb.Keys) ==> mapc[k] == mapa[k]; // no-set-op translation is easier for Dafny
-{
-    imap x : U | (x in mapa.Keys + mapb.Keys) :: if x in mapb then mapb[x] else mapa[x]
-}
 
 datatype Option<V> = None | Some(value:V)
 
